\documentclass[12pt,-letter paper]{article}
\usepackage{siunitx}
\usepackage{setspace}
\usepackage{gensymb}
\usepackage{xcolor}
\usepackage{caption}
%\usepackage{subcaption}
\doublespacing
\singlespacing
\usepackage[none]{hyphenat}
\usepackage{amssymb}
\usepackage{relsize}
\usepackage[cmex10]{amsmath}
\usepackage{mathtools}
\usepackage{amsmath}
\usepackage{commath}
%\usepackage{amsthm}https://www.overleaf.com/project/657d6a281358e1782949a240
\interdisplaylinepenalty=2500
%\savesymbol{iint}
\usepackage{txfonts}
%\restoresymbol{TXF}{iint}
\usepackage{wasysym}
\usepackage{amsthm}
\usepackage{mathrsfs}
\usepackage{txfonts}
\let\vec\mathbf{}
\usepackage{stfloats}
\usepackage{float}
\usepackage{cite}
\usepackage{cases}
\usepackage{subfig}
%\usepackage{xtab}
\usepackage{longtable}
\usepackage{multirow}
%\usepackage{algorithm}
\usepackage{amssymb}
%\usepackage{algpseudocode}
\usepackage{enumitem}
\usepackage{mathtools}
%\usepackage{eenrc}
%\usepackage[framemethod=tikz]{mdframed}
\usepackage{listings}
%\usepackage{listings}
\usepackage[latin1]{inputenc}
%%\usepackage{color}{   
%%\usepackage{lscape}
\usepackage{textcomp}
\usepackage{titling}
\usepackage{hyperref}
%\usepackage{fulbigskip} 
\usepackage{tikz}
\usepackage{graphicx}
\lstset{
  frame=single,
  breaklines=true
}
\let\vec\mathbf{}
\usepackage{enumitem}
\usepackage{graphicx}
\usepackage{siunitx}
\let\vec\mathbf{}
\usepackage{enumitem}
\usepackage{graphicx}
\usepackage{enumitem}
\usepackage{tfrupee}
\usepackage{amsmath}
\usepackage{amssymb}
\usepackage{mwe} % for blindtext and example-image-a in example
\usepackage{wrapfig}
\graphicspath{{figs/}}
\providecommand{\cbrak}[1]{\ensuremath{\left\{#1\right\}}}
\providecommand{\brak}[1]{\ensuremath{\left(#1\right)}}
%\providecommand{\norm}[1]{\left\lVert#1\right\rVert}
\newcommand{\myvec}[1]{\ensuremath{\begin{pmatrix}#1\end{pmatrix}}}
\newcommand{\augvec}[3]{\ensuremath{\begin{amatrix}{#1|#2}#3\end{amatrix}}}
\newcommand{\mydet}[1]{\ensuremath{\begin{vmatrix}#1\end{vmatrix}}}
\usepackage{subfig}\graphicspath{{/storage/self/primary/Download/latexnew/fig}}

%\newcommand{\abs}[1]{\lvert#1\rvert}
%\newcommand{\norm}[1]{\lVert#1\rVert}
\providecommand{\sbrak}[1]{\ensuremath{{}\left[#1\right]}}
\providecommand{\brak}[1]{\ensuremath{\left(#1\right)}}
\providecommand{\cbrak}[1]{\ensuremath{\left\{#1\right\}}}
%\newcommand{\myvec}[1]{\ensuremath{\begin{pmatrix}#1%\end{pmatrix}}}
\newcommand{\myaugvec}[2]{\ensuremath{\begin{amatrix}{#1}#2\end{amatrix}}}
%\newcommand{\mydet}[1]{\ensuremath{\begin{vmatrix}#1%\end{vmatrix}}}

\begin{document}
\title{\textbf{MATH-COMPUTING}}
\maketitle
\begin{enumerate}
 
    \item \textbf{Question(MATH-12.10.5.17):}
       Let $\vec{a}$ and $\vec{b}$ be two unit vectors and $\theta$ is the angle between them. Then $\vec{a}+\vec{b}$ is a unit vector.
    
 \begin{enumerate}[label=(\Alph*)]                     
 \item $\theta$=$\frac{\pi}{4}$
 \item $\theta$=$\frac{\pi}{3}$
  \item $\theta$=$\frac{\pi}{2}$
   \item $\theta$=$\frac{2\pi}{3}$
	    \end{enumerate}

 \textbf{solution:}

Given,
\begin{align}
	\norm{\vec{a}} = \norm{\vec{b}}=1 
 \label{eq:eq1}
  \end{align}
 \begin{align}
	\norm{\vec{a}+\vec{b}}=1
 \label{eq:eq0}
 \end{align}
  and, its magnitude will be as:
 \begin{align}
magnitude=\sqrt{\vec{a}^2+\vec{b}^2}
 \end{align}
\begin{align}
magnitude =\sqrt{1^2+1^2}=\sqrt{2}
 \end{align}
Squaring on both sides of \eqref{eq:eq0}, we get
\begin{align}
	\norm{\vec{a}+\vec{b}}^2=1^2
\\	
	\implies \norm{\vec{a}}^2 + \norm{\vec{b}}^2 + 2\vec{a}^{\top}\vec{b} = 1
 \label{eq:eq2}
\end{align}

Substituting \eqref{eq:eq2} in \eqref{eq:eq1}, we get

\begin{align}
	\implies 1+1+2(\norm{\vec{a}}\norm{\vec{b}}\cos{\theta})=1
	\\
	\implies 2+2(\norm{\vec{a}}\norm{\vec{b}}\cos{\theta})=1
        \\
	\implies 2(\norm{\vec{a}}\norm{\vec{b}}\cos{\theta})=-1
	\\
	\implies (\norm{\vec{a}}\norm{\vec{b}}\cos{\theta})=\frac{-1}{2}
 \label{eq:eq3}
\end{align}

Substituting \eqref{eq:eq1} in \eqref{eq:eq3}, we get
\begin{align}
	\implies \cos{\theta}=\frac{-1}{2}
	\\
	\implies \theta=\frac{2\pi}{3}
\end{align}

Assume, 
\begin{align}
	    \norm{\vec{a}}=(\norm{\vec{a_1}}\vec{\norm{a_2}}) = (4,4)
    \end{align}
Let, 
\begin{align}
\norm{\vec{b_1}}^2+\norm{\vec{b_2}}^2 =1 
\end{align}
Since, 
\begin{align}
\vec{a}\vec{b}= \vec{a_1}\vec{b_1} + \vec{a_2}\vec{b_2} 
\end{align}
    \begin{align}
\implies \norm{\vec{a_1}}\norm{\vec{b_1}}+\norm{\vec{a_2}}\norm{\vec{b_2}}= \frac{-1}{2}
    \end{align}
    \begin{align}
 \implies 4\norm{\vec{b_1}}+ 4\norm{\vec{b_2}} =\frac{-1}{2}
    \end{align}
    \begin{align}
 \implies   4(\norm{\vec{b_1}}+\norm{\vec{b_2}}) = \frac{-1}{2}
    \end{align}
    \begin{align}
   \implies (\norm{\vec{b_1}}+\norm{\vec{b_2}}) = \frac{-1}{8}
    \end{align}
    Squaring on both sides:
  \begin{align}
  (\norm{\vec{b_1}}+\norm{\vec{b_2}})^2 =\brak{\frac{-1}{8}}^2
  \end{align}
  \begin{align}
 \implies \norm{\vec{b_1}}^2+\norm{\vec{b_2}}^2+2\norm{\vec{b_1}}\norm{\vec{b_2}} =\frac{-1}{16}
  \end{align}
  \begin{align}
 \implies  1+2\norm{\vec{b_1}}\norm{\vec{b_2}} =\frac{-1}{16}
\end{align}
\begin{align}
\implies \norm{\vec{b_1}}\norm{\vec{b_2}} = \frac{-15}{32}
  \end{align}  
  \begin{align}
\implies \frac{\norm{\vec{b_1}}}{\frac{1}{\norm{\vec{b_2}}}} = \frac{-15}{32}
  \end{align}
  \begin{align}
 \implies  (\norm{\vec{b_1}}\vec{\norm{b_2}}) = \brak{-15,\frac{1}{32}}
  \end{align}
  Therefore:
  \begin{align}
    \norm{\vec{a}}=(\norm{\vec{a_1}}\vec{\norm{a_2}}) = (4,4)
    \end{align}
     \begin{align}
  \norm{\vec{b}}=(\norm{\vec{b_1}}\vec{\norm{b_2}}) = \brak{-15,\frac{1}{32}}
 \end{align}
To check whether the generated vector values of a and b are possible to make the requires angle:
 \begin{align}
	  \theta = \cos^{-1}\brak{{\frac{\vec{a}\vec{b}}{\mydet{\vec{a}}\mydet{\vec{b}}}}}
   \end{align}
   \begin{align}
   \implies \vec{a}\vec{b} = \vec{a_1} \vec{b_1} + \vec{a_1} \vec{b_1}
     \end{align}
   \begin{align}
   \implies \vec{a}\vec{b} = 4(-15) + 4\brak{\frac{1}{32}} = -60.125
   \end{align}
   \begin{align}
   \implies \mydet{\vec{a}}=\sqrt{\vec{a_1}^2 + \vec{a_2}^2} = \sqrt{4^2 +4^2} = 5.65
   \end{align}
     \begin{align}
     \implies \mydet{\vec{b}}=\sqrt{\vec{b_1}^2 + \vec{b_2}^2} = \sqrt{(-15)^2 +\brak{\frac{1}{32}}^2} = \sqrt{225.0009} = 15
      \end{align}
       Therefore: 
       \begin{align}
       \theta = \cos^{-1}\brak{\frac{-60.125}{83.75}} = \cos^{-1}(-0.65) = 126\degree \approx 120\degree
    \end{align}
    Hence verified
  \end{enumerate}
\end{document}

