\documentclass[11pt]{book}
\usepackage{gvv-book}
\usepackage{gvv}
\usepackage[sectionbib,authoryear]{natbib}
\setcounter{secnumdepth}{3}
\setcounter{tocdepth}{2}
\makeindex

\begin{document}
\frontmatter
\tableofcontents
\setcounter{page}{1}
\mainmatter
\chapter{Triangle}
Consider a triangle with vertices
\begin{align}
\label{eq:tri-pts}
\vec{A}=\myvec{-3 \\ -5},\,
\vec{B}=\myvec{3\\-5},\,
	\vec{c}=\myvec{-4\\-3},\,
\end{align}

\section{Vectors}
\section{median}


\begin{enumerate}[label=\thesection.\arabic*.,ref=\thesection.\theenumi]
\numberwithin{equation}{enumi}

%Question 1.2.1:
\item  If $\vec{D}$ divides $BC$ in the ratio $k : 1$,
		\begin{align}
			\vec{D}= \frac{k\vec{C}+\vec{B}}{k+1}
		\end{align}
Find the mid points $\vec{D}, \vec{E}, \vec{F}$ of the sides $BC, CA$ and $AB$ respectively.\\
If $\vec{D}$ divides $BC$ in the ratio $k : 1$,
\begin{align}
\vec{D}= \frac{k\vec{C}+\vec{B}}{k+1}
\end{align}
Find the mid points $\vec{D}, \vec{E}, \vec{F}$ of the sides $BC, CA$ and $AB$ respectively.
\newline
Given:
\begin{align}
\vec{A} &= \myvec{1\\3\\}\\
\vec{B} &= \myvec{-3\\0\\}\\
\vec{C} &= \myvec{0\\4\\}
\end{align}

\solution
Since $\vec{D}$ is the midpoint of $BC$,
\begin{align}
k &= 1\\
\implies \vec{D} &= \frac{\vec{C} + \vec{B}}{2}\\
&= \frac{1}{2}\myvec{-3\\4}
\end{align}
Similarly,
\begin{align}
\vec{E} &= \frac{\vec{A} + \vec{C}}{2}\\
&= \frac{1}{2}\myvec{1\\7}\\
\vec{F} &= \frac{\vec{A} + \vec{B}}{2}\\
&= \myvec{-3\\3}
\end{align}
\begin{figure}[H]
\centering
\includegraphics[width=\columnwidth]{/sdcard/hima//geometry/figs/median2.jpg}
\caption{Triangle ABC with midpoints D,E and F}
\end{figure}  

%Question 1.2.2:
\item Find the equations of $AD, BE$ and $CF$.\\
\\ \solution:
$\vec{D}$,$\vec{E}$,$\vec{F}$ are the midpoints of $BC$,$CA$,$AB$ respectively, then\\
\begin{align}
 \vec{D} &=  \myvec{\frac{-3}{2}\\2}\\
\vec{E} &=  \myvec{\frac{1}{2}\\\frac{7}{2}}\\
 \vec{F} &=  \myvec{\frac{-3}{2}\\\frac{3}{2}}\\
\end{align}
\begin{enumerate}

 \item The normal equation for the median $AD$ is
  \begin{align}
    \vec{n}^{\top}\myvec{\vec{x}-\vec{A}}&=0\\
    \implies
    \vec{n}^{\top}\vec{x}&=\vec{n}^{\top}\vec{A}
  \end{align}
 We have to find the $\vec{n}$ so that we can find $\vec{n}^{\top}$.
 Since,
\begin{align}
  \vec{n} &= \myvec{0 & 1\\
  -1 & 0}\vec{m}
\end{align}
Here $\vec{m} = \vec{D}- \vec{A}$ for median $AD$
\begin{align}
\vec{m}&=\myvec{\frac{-3}{2}\\ 2} - \myvec{1\\3}\\
       &=\myvec{\frac{-5}{2}\\-1}
\end{align}
Since,
\begin{align}
  \vec{n} &= \myvec{0 & 1\\
  -1 & 0}\vec{m}\\
\implies
\vec{n} &= \myvec{0 & 1\\
  -1 & 0}\myvec{\frac{-5}{2}\\-1}\\
        &= \myvec{-1 \\\frac{5}{2}}
\end{align}
Hence the normal equation of median $AD$ is 
\begin{align}
    \myvec{-1 & \frac{5}{2}}\vec{x}&=\myvec{-1 & \frac{5}{2}}\myvec{1\\3}\\
    \implies
    \myvec{-1 & \frac{5}{2}}\vec{x}&=\frac{13}{2}
\end{align}

\item The normal equation for the median $BE$ is
\begin{align}
\vec{n}^{\top}\myvec{\vec{x}-\vec{B}}&=0\\
\implies
\vec{n}^{\top}\vec{x}&=\vec{n}^{\top}\vec{B}
\end{align}
Here $\vec{m} = \vec{E}- \vec{B}$ for median $BE$
\begin{align}
\vec{m}&=\myvec{\frac{1}{2}\\\frac{7}{2}} - \myvec{-3\\0}\\
       &=\myvec{\frac{7}{2}\\\frac{7}{2}}
\end{align}
Since,
\begin{align}
  \vec{n} &= \myvec{0 & 1\\
  -1 & 0}\vec{m}\\
\implies
\vec{n} &= \myvec{0 & 1\\
  -1 & 0}\myvec{\frac{7}{2}\\\frac{7}{2}}\\
        &= \myvec{\frac{7}{2}\\ \frac{-7}{2}}
\end{align}
Hence the normal equation of median $BE$ is 
\begin{align}
    \myvec{\frac{7}{2} & \frac{-7}{2}}\vec{x}&=\myvec{\frac{7}{2} & \frac{-7}{2}}\myvec{-3\\0}\\
\implies
    \myvec{\frac{7}{2}& \frac{-7}{2}}\vec{x}&=\frac{-21}{2}
\end{align}

\item The normal equation for the median $CF$ is
\begin{align}
\vec{n}^{\top}\myvec{\vec{x}-\vec{C}}&=0\\
\implies
\vec{n}^{\top}\vec{x}&=\vec{n}^{\top}\vec{C}
\end{align}
Here $\vec{m} = \vec{F}- \vec{C}$ for median $CF$
\begin{align}
\vec{m}&=\myvec{\frac{-3}{2}\\\frac{3}{2}} - \myvec{0\\4}\\
       &=\myvec{-1\\\frac{-5}{2}}
\end{align}
Since,
\begin{align}
  \vec{n} &= \myvec{0 & 1\\
  -1 & 0}\vec{m}\\
\implies
\vec{n} &= \myvec{0 & 1\\
  -1 & 0}\myvec{-1\\ \frac{-5}{2} }\\
        &= \myvec{\frac{-5}{2} \\ 1}
\end{align}
Hence the normal equation of median $CF$ is 
\begin{align}
    \myvec{\frac{-5}{2} & 1 }\vec{x}&=\myvec{\frac{-5}{2} & 1}\myvec{0\\4}\\
\implies
    \myvec{\frac{-5}{2} & 1}\vec{x}&=-4
\end{align}
\end{enumerate}
\begin{figure}
\includegraphics[width=\columnwidth]{/sdcard/hima/geometry/figs/median3.jpg'}
\caption{ Medians $AD$ , $BE$ and $CF$}
\label{fig: medians}
\end{figure}


%Question 1.2.3:
\item Find the intersection $\vec{G}$ of $BE$ and $CF$
\\ 
\solution 
$\vec{A},\vec{B}$ and $\vec{C}$ are vertices of triangle:
\begin{align}
    \vec{A} &= \myvec{1 \\3} \\
    \vec{B} &= \myvec{-3 \\ 0} \\
    \vec{C} &= \myvec{0 \\4}
\end{align}
Since $\vec{E}$ and $\vec{F}$ are midpoints of $CA$ and $AB$,
\begin{align}
    \vec{E} &= \frac{\vec{A} + \vec{C}}{2} \\
	&= \myvec{\frac{1}{2} \\\frac{7}{2}}\\
    \vec{F} &= \frac{\vec{B} + \vec{A}}{2} \\ 
    &= \myvec{ \frac{-3}{2} \\ \frac{3}{2}}
\end{align}
The line $BE$ in vector form is given by
\begin{align}
\myvec{\frac{7}{2}& \frac{-7}{2}} \vec{x} &= \myvec{\frac{-21}{2}}
\label{eq:1.2.3,8}
\end{align}
The line $CF$ in vector form is given by
\begin{align}
\myvec{ \frac{-5}{2}&-1} \vec{x} &= \myvec{-4}
\label{eq:1.2.3,9}
\end{align}
From \eqref{eq:1.2.3,8} and \eqref{eq:1.2.3,9} the augmented matrix is:
\begin{align}
\myvec{
\frac{7}{2} & \frac{-7}{2} & \frac{-21}{2} \\
\frac{-5}{2} & -1 & -4
}
\end{align}
Solve for $\vec{x}$ using Gauss-Elimination method:
\begin{align}
    \label{eq:matrowoperations}
 \myvec{
\frac{7}{2}& \frac{-7}{2} & \frac{-21}{2} \\
\frac{-5}{2} & -1 & -4
}
\xleftrightarrow[]{R_2 \leftarrow R_2+2R_1}
    \myvec{
    \frac{7}{2}& \frac{-7}{2} & \frac{-21}{2}
    \\
    \frac{9}{2} & -8 & -25 
    }
    \\
     \xleftrightarrow[]{R_2\leftarrow R_2/9}
    \myvec{
    \frac{7}{2} & \frac{-7}{2} & \frac{-21}{2}
    \\
    \frac{1}{2} & \frac{-8}{9} & \frac{-25}{9} 
    }
    \\
     \xleftrightarrow[]{R_1\leftarrow R_1-\frac{13}{2}R_2}
    \myvec{
    \frac{1}{4} & \frac{-27}{4} & \frac{-55}{4}
    \\
    \frac{1}{2} & \frac{-8}{9} & \frac{-25}{9}
    }
\end{align} 
Therefore, 
\begin{align}
\vec{G} = \myvec{\frac{-55}{4} \\ \frac{-25}{9}}
\end{align}
From Fig. \ref{fig:Triangle101}, We can see that $\vec{G}=\myvec{\frac{-55}{4}\\ \frac{-25}{9}}$ is the intersection of $BE$ and $CF$
\begin{figure}[h]
\centering
\includegraphics[width=\columnwidth]{/sdcard/hima/geometry/figs/median2.jpg'}
\caption{$G$ is the centroid of triangle $ABC$}
\label{fig:Triangle101}
\end{figure}



%Question 1.2.4:
\item Verify that 
		\begin{align}
			\frac{BG}{GE} = 
			\frac{CG}{GF} =
			\frac{AG}{GD} =2 
		\end{align}\\
Question 1.2.4:Verify that 
\begin{align}
		\frac{BG}{GE} = 
		\frac{CG}{GF} =
		\frac{AG}{GD} = 2 
\end{align}
\solution In order to verify the above equation we first need to find $\vec{G}$.$\vec{G}$ is the intersection of $BE$ and $CF$,Using the value of $\vec{G}$ from (1.2.3).
\begin{align}
		\vec{G} = \myvec{\frac{-55}{4} \\ \frac{-25}{9}}
\end{align}
Also,We know that $\vec{D}, \vec{E}$ and $\vec{F}$ are midpoints of $BC, CA$ and $AB$ respectively from (1.2.1).
\begin{align}
		\vec{D} = \myvec{\frac{-3}{2} \\ 2},\,
		\vec{E} = \myvec{\frac{1}{2} \\ \frac{7}{2}},\,
		\vec{F} = \myvec{\frac{-3}{2} \\ \frac{3}{2}}
\end{align}
\begin{enumerate}
\item Calculating the ratio of $BG$ and $GE$,
\begin{align}
		\label{eq:tri-pts/4} \vec{G}-\vec{B} &= \myvec{\frac{-67}{4} \\ \frac{-25}{9}} \\
		\label{eq:tri-pts/5} \vec{E}-\vec{G} &= \myvec{\frac{57}{4} \\ \frac{113}{18}} \\
		\label{eq:tri-pts/6} \norm{\vec{G}-\vec{B}} &= \sqrt{\brak{\frac{-67}{4}}^2 + \brak{\frac{25}{9}}^{2}} &= \frac{\sqrt{288}}{3} \\
		\label{eq:tri-pts/7} \norm{\vec{E}-\vec{G}} &= \sqrt{\brak{\frac{57}{4}}^2 + \brak{\frac{113}{18}}^2} &= \frac{\sqrt{288}}{6} \\
		\label{eq:tri-pts/8}\frac{BG}{GE} &= \frac{\norm{\vec{G}-\vec{B}}}{\norm{\vec{E}-\vec{G}}} &= \frac{\frac{\sqrt{288}}{3}}{\frac{\sqrt{288}}{6}} &= 2  
\end{align}		
\item Calculating the ratio of $CG$ and $GF$,
\begin{align}
		\label{eq:tri-pts/9} \vec{G}-\vec{C} &= \myvec{\frac{-55}{4} \\ \frac{-61}{9}} \\
		\label{eq:tri-pts/10} \vec{F}-\vec{G} &= \myvec{\frac{51}{4} \\ \frac{77}{18}} \\
		\label{eq:tri-pts/11} \norm{\vec{G}-\vec{C}} &= \sqrt{\brak{\frac{-55}{4}}^{2} + \brak{\frac{-61}{9}}^{2}} &= \frac{\sqrt{800}}{3} \\  
		\label{eq:tri-pts/12} \norm{\vec{F}-\vec{G}} &= \sqrt{\brak{\frac{51}{4}}^{2} + \brak{\frac{77}{18}}^{2}} &= \frac{\sqrt{200}}{3} \\
		\label{eq:tri-pts/13}\frac{CG}{GF} &= \frac{\norm{\vec{G}-\vec{C}}}{\norm{\vec{F}-\vec{G}}} &= \frac{\frac{\sqrt{80}}{3}}{\frac{\sqrt{20}}{3}} &= 2		
\end{align}
\item Calculating the ratio of $AG$ and $GD$,
\begin{align}
		\label{eq:tri-pts/14} \vec{G}-\vec{A} &= \myvec{\frac{-59}{4} \\ \frac{-52}{9}} \\
		\label{eq:tri-pts/15} \vec{D}-\vec{G} &= \myvec{\frac{49}{4} \\ \frac{43}{9}} \\
		\label{eq:tri-pts/16} \norm{\vec{G}-\vec{A}} &= \sqrt{\brak{\frac{-59}{4}}^{2} + \brak{\frac{-52}{9}}^{2}} &= \frac{\sqrt{1280}}{4} \\
		\label{eq:tri-pts/17} \norm{\vec{D}-\vec{G}} &= \sqrt{\brak{\frac{49}{4}}^{2}+\brak{\frac{43}{9}}^{2}} &= \frac{\sqrt{1280}}{8} \\
		\label{eq:tri-pts/18}\frac{AG}{GD} &= \frac{\norm{\vec{G}-\vec{A}}}{\norm{\vec{D}-\vec{G}}} &= \frac{\frac{\sqrt{1290}}{4}}{\frac{\sqrt{1290}}{8}} &= 2 
\end{align}
\end{enumerate}

From \eqref{eq:tri-pts/8}, \eqref{eq:tri-pts/13}, \eqref{eq:tri-pts/18}
\begin{align}
		\frac{BG}{GE} = 
		\frac{CG}{GF} =
		\frac{AG}{GD} = 2
\end{align}
Hence verified.



%Question 1.2.5:
\item Show that $\vec{A}, \vec{G}$ and $\vec{D}$ are collinear.\\
\solution 
Given that,
\begin{align}
    \vec{A} = \myvec{1\\3}
    \quad
    \vec{B} &= \myvec{-3\\0}
    \quad
    \vec{C} = \myvec{0\\4}
\end{align}
We need to show that points $\vec{A},\vec{D},\vec{G}$ are collinear.
From Problem 1.2.3 We know that, The point $\vec{G}$ is 
\begin{align}
    \vec{G} &=\myvec{\frac{-55}{4}\\ \frac{-25}{9}}
\end{align}
And from Problem 1.2.1 We know that, The point $\vec{D}$ is 
\begin{align}
    \vec{D} &=\myvec{\frac{-3}{2}\\ 2}
\end{align}
In Problem 1.1.3, There is a theorem/law mentioned i.e.,

Points $\vec{A},\vec{D},\vec{G}$ are defined to be collinear if 
\begin{align}
    \text{rank}\myvec{
    1 & 1 & 1\\
    \vec{A} & \vec{D} & \vec{G} \\
    } &= 2 
\end{align} 
Using the above law/Theorem Let
\begin{align}
    \vec{R}&=\myvec{
    1 & 1 & 1
    \\
    1 & \frac{-3}{2} & \frac{-55}{4}
    \\
    3 & 2 & \frac{-25}{9}
    } 
\end{align} 
The matrix $\vec{R}$ can be row reduced as follows,
\begin{align}
    \label{eq:mat_row_operations}
    \myvec{
    1 & 1 & 1
    \\
    1 & \frac{-3}{2} & \frac{-55}{4}
    \\
    3 & 2 & \frac{-25}{9}
    }
     \xleftrightarrow[]{R_2 \leftarrow R_2+3R_1}
    \myvec{
    1 & 1 & 1
    \\
    4 & \frac{3}{2} & 13
    \\
    3 & 2 & \frac{-25}{9} 
    }
    \\
     \xleftrightarrow[]{R_2\leftarrow \frac{2}{5}R_2}
    \myvec{
    1 & 1 & 1
    \\
    \frac{8}{5} & \frac{3}{5} & \frac{26}{5}
    \\
    3 & 2 &  \frac{-25}{9}
    }
    \\
     \xleftrightarrow[]{R_3\leftarrow R_3-R_2}
    \myvec{
    1 & 1 & 1
    \\
    \frac{8}{5} & \frac{3}{5} & \frac{26}{5}
    \\
    \frac{7}{5} & \frac{7}{5} & \frac{-359}{45}
    }
\end{align}
Rank of above matrix is 2.\\
Hence, we proved that that points $\vec{A},\vec{D},\vec{G}$ are collinear.



%Question 1.2.6:
\item Verify that 
		\begin{align}
			\vec{G}=\frac{\vec{A}+\vec{B}+\vec{C}}{3}
		\end{align}
$\vec{G}$ is known as the {\em centroid} of $\triangle ABC$.\\
Verify that\\
\begin{align}
 \vec{G}=\frac{\vec{A}+\vec{B}+\vec{C}}{3}   
\end{align}
$\vec{G}$ is known as the \underline{centroid} of $\triangle$ABC 
SOLUTION:\\
let us first evaluate the R.H.S of the equation
\begin{equation}
\begin{split}
\label{eq:centroid}
    \vec{G}&= \frac{\myvec{1\\3}+\myvec{-3\\0}+\myvec{0\\4}}{3}\\    
    &= \myvec{\frac{1-3+0}{3} \\ \frac{3+0+4}{3}}\\
     &= \myvec{\frac{-2}{3}\\ \frac{7}{3}}
\end{split}
\end{equation}
Hence verified.


%Question 1.2.7: 
\item Verify that 
		\begin{align}
\vec{A}-\vec{F}=\vec{E}-\vec{D}
		\end{align}
The quadrilateral $AFDE$ is defined to be a parallelogram.\\
Question : Verify that 
\begin{align}
	\vec{A}-\vec{F} = \vec{E}-\vec{D}
\end{align}
The quadrilateral $AFDE$ is defined to be parallelogram
\\ \solution 
Given that,
\begin{align}
    \vec{A} = \myvec{1\\3}
    \quad
    \vec{B} &= \myvec{-3\\0}
    \quad
    \vec{C} = \myvec{0\\4}
\end{align}
From Problem 1.2.1 We know that, The point $\vec{D},\vec{E},\vec{F}$ is 
\begin{align}
    \vec{D} = \myvec{\frac{-3}{2}\\ 2 }
    \quad
    \vec{E} &= \myvec{\frac{1}{2}\\\frac{7}{2}}
    \quad
    \vec{F} = \myvec{-1\\ \frac{3}{2}}
\end{align}
Evaluating the R.H.S of the equation
\begin{align}
    \vec{A}-\vec{F}&=\myvec{1\\3}-\myvec{-1\\ \frac{3}{2} }\\
    &=\myvec{ 2 \\ \frac{3}{2} }
\end{align} 
Evaluating the L.H.S of the equation
\begin{align}
    \vec{E}-\vec{D}&=\myvec{1\\3}-\myvec{-1\\ \frac{3}{2} }\\
    &=\myvec{2 \\\frac{3}{2} }
\end{align}
Hence verified that, R.H.S = L.H.S i.e.,
\begin{align}
	\vec{A}-\vec{F} = \vec{E}-\vec{D}
\end{align}
From the fig\ref{fig:Triangle}, It is verified that $AFDE$ is a parallelogram
\begin{figure}
\centering
\includegraphics[width=\columnwidth]{/sdcard/hima/geometry/figs/median3.jpg}
\caption{$AFDE$ form a parallelogram in triangle ABC}
\label{fig:Triangle}
\end{figure}
\end{enumerate}














%\input{subsec/median}
%\section{Altitude}
%\section{Perpendicular Bisector}
%\section{Angle Bisector}

\end{document}
